lean/privacy/actions/action_spec.lean
@@ -85,22 +85,22 @@ def open_subchannel (crypto: Crypto) (inp: OpenSubchannelInput) (m: Memory) : Li
 -----------------
 
 structure CreateNoteInput where
-  (addralice kalice addrbob Kbob token i₀ i₁ r amount: ℕ)
+  (addralice kalice addrbob Kbob token i r amount: ℕ)
 
 abbrev CreateNoteInput.c (crypto: Crypto) (inp: CreateNoteInput) : ℕ :=
   crypto.hash [inp.addralice, inp.kalice, inp.addrbob, inp.Kbob]
 
 abbrev CreateNoteInput.note_id (crypto: Crypto) (inp: CreateNoteInput) : ℕ :=
-  crypto.hash [inp.c crypto, inp.token, inp.i₀, inp.i₁]
+  crypto.hash [inp.c crypto, inp.token, inp.i]
 
 abbrev CreateNoteInput.enc (crypto: Crypto) (inp: CreateNoteInput) : ℕ :=
-  (if inp.r = 1 then 0 else crypto.hash [inp.c crypto, inp.token, inp.i₀, inp.i₁, inp.r]) + inp.amount
+  (if inp.r = 1 then 0 else crypto.hash [inp.c crypto, inp.token, inp.i, inp.r]) + inp.amount
 
 def create_note (crypto: Crypto) (inp: CreateNoteInput) (m: Memory) : List ServerAction × Bool :=
   let c := inp.c crypto
   let note_id := inp.note_id crypto
   let subchannel_exists := m .SubchannelMarkers [crypto.hash [c, inp.addrbob, inp.Kbob, inp.token]] ≠ 0
-  let prev_note_exists := inp.i₁ = 0 ∨ m .Notes [crypto.hash [c, inp.token, inp.i₀, inp.i₁ - 1], 0] ≠ 0
+  let prev_note_exists := inp.i = 0 ∨ m .Notes [crypto.hash [c, inp.token, inp.i - 1], 0] ≠ 0
   ([
     .WriteOnce .Notes [note_id, 0] (crypto.pack inp.r (inp.enc crypto)),
     .Write .OpenNoteToken [note_id] (if inp.r = 1 then inp.token else 0),
@@ -110,23 +110,23 @@ def create_note (crypto: Crypto) (inp: CreateNoteInput) (m: Memory) : List Serve
       else
         .None
     ),
-  ], inp.r ≠ 0 ∧ prev_note_exists ∧ inp.i₀ < crypto.MAX_I₀ ∧ subchannel_exists ∧ (inp.r = 1 → inp.amount = 0))
+  ], inp.r ≠ 0 ∧ prev_note_exists ∧ subchannel_exists ∧ (inp.r = 1 → inp.amount = 0))
 
 -----------------
 -- Use Note --
 -----------------
 
 structure UseNoteInput where
-  (c addrbob kbob token i₀ i₁: ℕ)
+  (c addrbob kbob token i: ℕ)
   -- `amount` is not really an input since it can be computed from the memory and the other inputs.
   -- It is included here for convenience.
   (amount: ℕ)
 
 abbrev UseNoteInput.nullifier (crypto: Crypto) (inp: UseNoteInput) : ℕ :=
-  crypto.hash [inp.c, inp.token, inp.i₀, inp.i₁, inp.kbob]
+  crypto.hash [inp.c, inp.token, inp.i, inp.kbob]
 
 abbrev UseNoteInput.note_id (crypto: Crypto) (inp: UseNoteInput) : ℕ :=
-  crypto.hash [inp.c, inp.token, inp.i₀, inp.i₁]
+  crypto.hash [inp.c, inp.token, inp.i]
 
 abbrev UseNoteInput.Kbob (crypto: Crypto) (inp: UseNoteInput) : ℕ :=
   crypto.priv_to_pub inp.kbob
@@ -134,7 +134,7 @@ abbrev UseNoteInput.Kbob (crypto: Crypto) (inp: UseNoteInput) : ℕ :=
 def use_note (crypto: Crypto) (inp: UseNoteInput) (m: Memory) : List ServerAction × Bool :=
   let subchannel_exists := m .SubchannelMarkers [crypto.hash [inp.c, inp.addrbob, inp.Kbob crypto, inp.token]] ≠ 0
   let r := m .Notes [inp.note_id crypto, 0]
-  let dec_amount := note_amount crypto m (inp.note_id crypto) inp.c inp.token inp.i₀ inp.i₁
+  let dec_amount := note_amount crypto m (inp.note_id crypto) inp.c inp.token inp.i
   ([
     .WriteOnce .Nullifiers [inp.nullifier crypto] 1,
   ], subchannel_exists ∧ r ≠ 0 ∧ dec_amount = inp.amount ∧ inp.kbob ∈ crypto.PrivateKeys ∧ inp.amount ≠ 0)
