lean/privacy/amounts/amounts.lean
@@ -412,7 +412,7 @@ def spent_notes_from_scan
   (addrbob: ℕ) (kbob: crypto.PrivateKeys) (token: ℕ) : Finset ScannedNote :=
   scan_notes_for_recipient₀ context addrbob kbob
   |>.filter (λ sn ↦ sn.token = token)
-  |>.filter (λ sn ↦ m .Nullifiers [crypto.hash [sn.c, sn.token, sn.i₀, sn.i₁, kbob]] ≠ 0)
+  |>.filter (λ sn ↦ m .Nullifiers [crypto.hash [sn.c, sn.token, sn.i, kbob]] ≠ 0)
   |>.toFinset
 
 theorem spent_notes_from_scan' {crypto: Crypto} {rm: ReachableMemory crypto}
@@ -575,7 +575,7 @@ def spent_notes
   (
     scan_notes_for_recipient₀ context addrbob kbob
     |>.filter (λ sn ↦ sn.token = token)
-    |>.filter (λ sn ↦ m .Nullifiers [crypto.hash [sn.c, sn.token, sn.i₀, sn.i₁, kbob]] ≠ 0)
+    |>.filter (λ sn ↦ m .Nullifiers [crypto.hash [sn.c, sn.token, sn.i, kbob]] ≠ 0)
   )
 
 def spent_notes_ex
@@ -584,7 +584,7 @@ def spent_notes_ex
   (
     scan_notes_for_recipient context addrbob kbob
     |>.filter (λ sn ↦ sn.token = token)
-    |>.filter (λ sn ↦ m .Nullifiers [crypto.hash [sn.c, sn.token, sn.i₀, sn.i₁, kbob]] ≠ 0)
+    |>.filter (λ sn ↦ m .Nullifiers [crypto.hash [sn.c, sn.token, sn.i, kbob]] ≠ 0)
   )
 
 theorem spent_notes_ex_eq_spent_notes
@@ -652,7 +652,7 @@ theorem sum_create_note_use_note
     (
       scan_notes_for_recipient₀ (.from rm) bob.addr bob.k
       |>.filter (λ sn ↦ sn.token = token)
-      |>.filter (λ sn ↦ rm.m .Nullifiers [crypto.hash [sn.c, sn.token, sn.i₀, sn.i₁, bob.k]] = 0)
+      |>.filter (λ sn ↦ rm.m .Nullifiers [crypto.hash [sn.c, sn.token, sn.i, bob.k]] = 0)
       |>.map (λ sn ↦ sn.amount crypto rm)
       |>.sum
     ) := by
@@ -660,8 +660,8 @@ theorem sum_create_note_use_note
   set ℓ := scan_notes_for_recipient₀ (.from rm) bob.addr bob.k
   set f_token := λ sn: ScannedNote ↦ sn.token = token
   set amount := λ sn: ScannedNote ↦ sn.amount crypto rm
-  let f_spent := λ sn: ScannedNote ↦ (rm.m .Nullifiers [crypto.hash [sn.c, sn.token, sn.i₀, sn.i₁, bob.k]] ≠ 0)
-  let f_unspent := λ sn: ScannedNote ↦ (rm.m .Nullifiers [crypto.hash [sn.c, sn.token, sn.i₀, sn.i₁, bob.k]] = 0)
+  let f_spent := λ sn: ScannedNote ↦ (rm.m .Nullifiers [crypto.hash [sn.c, sn.token, sn.i, bob.k]] ≠ 0)
+  let f_unspent := λ sn: ScannedNote ↦ (rm.m .Nullifiers [crypto.hash [sn.c, sn.token, sn.i, bob.k]] = 0)
 
   have neg_f_spent : (λ sn ↦ decide ¬f_spent sn) = (λ sn ↦ decide (f_unspent sn)) := by
     ext x; classical simp [f_spent, f_unspent]
