lean/privacy/notes/contiguous.lean
@@ -2,9 +2,9 @@ import privacy.utils
 import privacy.actions
 import privacy.notes.notes
 
--- The i₁-s of notes for given (c, token, i₀) form a contiguous range [0, i₁_bound).
-theorem notes_contiguous {crypto: Crypto} {rm: ReachableMemory crypto} (c token i₀: ℕ) :
-  ∃ i₁_bound, ∀ i₁, i₁ < i₁_bound ↔ note_exists rm (crypto.hash [c, token, i₀, i₁]) := by
+-- The i-s of notes for given (c, token) form a contiguous range [0, i_bound).
+theorem notes_contiguous {crypto: Crypto} {rm: ReachableMemory crypto} (c token: ℕ) :
+  ∃ i_bound, ∀ i, i < i_bound ↔ note_exists rm (crypto.hash [c, token, i]) := by
   revert rm
   apply ReachableMemory.induction
   case inv₀ => use 0; intros; simp [ReachableMemory.m, note_exists]
@@ -12,40 +12,40 @@ theorem notes_contiguous {crypto: Crypto} {rm: ReachableMemory crypto} (c token 
   intro action rm ih success
   cases action
   case CreateNote inp =>
-    obtain ⟨i₁_bound, ih⟩ := ih
+    obtain ⟨i_bound, ih⟩ := ih
     let info := create_note_info crypto inp rm success
     rw [ReachableMemory.add_m, run_action, ←info.h_m']
 
-    by_cases h₀ : c = inp.c crypto ∧ token = inp.token ∧ i₀ = inp.i₀
+    by_cases h₀ : c = inp.c crypto ∧ token = inp.token
     case pos =>
-      use i₁_bound + 1
-      intro i₁
+      use i_bound + 1
+      intro i
       unfold note_exists
 
-      have h_inp_i₁_not_small : ¬inp.i₁ < i₁_bound := by
+      have h_inp_i_not_small : ¬inp.i < i_bound := by
         by_contra h'
-        have := (ih inp.i₁).1 h'
+        have := (ih inp.i).1 h'
         unfold note_exists at this
         simp only [h₀] at this
         have := info.old_value_was_zero
         contradiction
 
-      have h_inp_i₁_not_big : ¬inp.i₁ > i₁_bound := by
+      have h_inp_i_not_big : ¬inp.i > i_bound := by
         cases info.prev_note_exists
         case inl h_prev => omega
         case inr h_prev =>
-          have := (ih (inp.i₁ - 1)).2 (by
+          have := (ih (inp.i - 1)).2 (by
             unfold note_exists
             simp only [h₀]
             exact h_prev
           )
           omega
 
-      have h_i₁ : i₁_bound = inp.i₁ := by omega
+      have h_i : i_bound = inp.i := by omega
 
-      by_cases h₁ : i₁ = inp.i₁
+      by_cases h₁ : i = inp.i
       case pos =>
-        rw [h₁, h_i₁, h₀.1, h₀.2.1, h₀.2.2, info.memory_diff₀]
+        rw [h₁, h_i, h₀.1, h₀.2, info.memory_diff₀]
         simp only [lt_add_iff_pos_right, Nat.lt_one_iff, pos_of_gt, ne_eq, true_iff]
         exact crypto.pack_nz info.r_ne_zero
       case neg =>
@@ -56,22 +56,22 @@ theorem notes_contiguous {crypto: Crypto} {rm: ReachableMemory crypto} (c token 
           injections h'
           contradiction
         ) (by simp)]
-        have := ih i₁
+        have := ih i
         simp only [note_exists] at this
         rw [←this]
         omega
     case neg =>
-      use i₁_bound
-      intro i₁
-      replace h := ih i₁
+      use i_bound
+      intro i
+      replace h := ih i
       unfold note_exists
-      have : crypto.hash [c, token, i₀, i₁] ≠
-        crypto.hash [inp.c crypto, inp.token, inp.i₀, inp.i₁] := by
+      have : crypto.hash [c, token, i] ≠
+        crypto.hash [inp.c crypto, inp.token, inp.i] := by
         by_contra h₁
         apply crypto.h_hash at h₁
         injections h₁
-        rename_i h₁₀ h₁₁ h₁₂ h₁₃
-        exact h₀ ⟨h₁, h₁₀, h₁₁⟩
+        rename_i h₁₀ h₁₁
+        exact h₀ ⟨h₁, h₁₀⟩
       rw [info.no_change _ _ (by simp [this]) (by simp)]
       exact h
 
